More work on decompile_compile theorem

sandbox/Compile.v
@@ -1,3 +1,4 @@
+Require Import Coq.Program.Equality.
 Require Import Codes.
 Require Import Combinators.
 Require Import DeBruijn.
@@ -39,8 +40,8 @@ Section compiles_to_compile.
     repeat match goal with
     | [ H' : forall c : _, compiles_to ?t c -> compile ?t = c |- _] =>
       match goal with
-      | [ H : compiles_to ?t ?c' |- _] =>
-        apply H' in H; rewrite H; clear H; simpl
+      | [ H : compiles_to t _ |- _] =>
+        apply H' in H; rewrite H; clear H H'; simpl
       end
     end;
     auto.
@@ -66,9 +67,7 @@ Fixpoint decompile {Var : Set} (c : Code Var) : Term Var :=
   | BOT%code => BOT
   | (J * x * y)%code => decompile x || decompile y
   | (R * x * y)%code => decompile x (+) decompile y
-  | I => 
-      let v := VAR None in
-      LAMBDA v
+  | I => DeBruijn.I
   | (K * x)%code =>
       let x' := protect (decompile x) in
       LAMBDA x'
@@ -99,20 +98,107 @@ Fixpoint decompile {Var : Set} (c : Code Var) : Term Var :=
   | R => DeBruijn.K (+) DeBruijn.F
   end.
 
+Inductive decompiles_to {Var : Set} : Code Var -> Term Var -> Prop :=
+  | decompiles_to_top : decompiles_to TOP%code TOP
+  | decompiles_to_bot : decompiles_to BOT%code BOT
+  | decompiles_to_join x x' y y' :
+     decompiles_to x x' -> decompiles_to y y' ->
+     decompiles_to (J * x * y)%code (x' || y')
+  | decompiles_to_rand x x' y y' :
+     decompiles_to x x' -> decompiles_to y y' ->
+     decompiles_to (R * x * y)%code (x' (+) y')
+  | decompiles_to_i : decompiles_to I DeBruijn.I
+  | decompiles_to_k1 x x' :
+      decompiles_to x x' ->
+      let x'' := protect x' in
+      decompiles_to (K * x)%code (LAMBDA x'')
+  | decompiles_to_b2 x x' y y' :
+      decompiles_to x x' ->
+      decompiles_to y y' ->
+      let x'' := protect x' in
+      let y'' := protect y' in
+      let v := VAR None in
+      decompiles_to (B * x * y)%code (LAMBDA (x'' * (y'' * v)))
+  | decompiles_to_c2 x x' y y' :
+      decompiles_to x x' ->
+      decompiles_to y y' ->
+      let x'' := protect x' in
+      let y'' := protect y' in
+      let v := VAR None in
+      decompiles_to (C * x * y)%code (LAMBDA (x'' * v * y''))
+  | decompiles_to_s2 x x' y y' :
+      decompiles_to x x' ->
+      decompiles_to y y' ->
+      let x'' := protect x' in
+      let y'' := protect y' in
+      let v := VAR None in
+      decompiles_to (S * x * y)%code (LAMBDA (x'' * v * (y'' * v)))
+  | decompiles_to_app x x' y y':
+      decompiles_to x x' ->
+      decompiles_to y y' ->
+      decompiles_to (x * y)%code (x' * y')
+  | decompiles_to_var v : decompiles_to (code_var v) (term_var v)
+  (* these cases never arise as [decompile (compile t)] *)
+  | decompiles_to_k : decompiles_to K DeBruijn.K
+  | decompiles_to_b : decompiles_to B DeBruijn.B
+  | decompiles_to_c : decompiles_to C DeBruijn.C
+  | decompiles_to_s : decompiles_to S DeBruijn.S
+  | decompiles_to_j : decompiles_to J (DeBruijn.K || DeBruijn.F)
+  | decompiles_to_r : decompiles_to R (DeBruijn.K (+) DeBruijn.F)
+.
+Hint Constructors decompiles_to.
+
+Section decompiles_to_decompile.
+  Local Ltac decompiles_to_decompiles :=
+    simpl;
+    repeat match goal with
+    | [ H' : forall c : _, decompiles_to c ?t -> decompile c = ?t |- _] =>
+      match goal with
+      | [ H : decompiles_to _ t |- _] =>
+        apply H' in H; rewrite H; clear H H'; simpl
+      end
+    end;
+    auto.
+
+  Lemma decompiles_to_decompile (Var : Set) (c : Code Var) (t : Term Var) :
+    decompiles_to c t <-> decompile c = t.
+  Proof.
+    split.
+    - intro H; induction t; inversion H; decompiles_to_decompiles;
+      admit.
+    - intro H; dependent induction c;
+      try (simpl in H; rewrite <- H; auto; reflexivity).
+      admit.
+  Qed.
+End decompiles_to_decompile.
+
 
 Section decompile_compile.
   Local Ltac decompile_compile :=
     simpl;
     repeat match goal with
-    | [H : decompile (compile ?x) = ?x |- _] => rewrite H; clear H; simpl
-    end.
+    | [H : decompile (compile ?x) = ?x |- _] => rewrite H; simpl
+    end;
+    auto.
+
+  Local Ltac compiles_to :=
+    simpl;
+    repeat match goal with
+    | [H : compiles_to ?t ?c |- _] =>
+        apply compiles_to_compile in H; try rewrite H
+    end;
+    auto.
 
   Lemma decompile_compile_normal (Var : Set) (t : Term Var) :
-   normal t -> decompile (compile t) = t.
+    normal t -> decompile (compile t) = t.
   Proof.
-    intro Hn; induction Hn; decompile_compile; auto.
-    - case_eq (compile x); intros; try (compute; reflexivity);
-      admit.
+    intro Hn; induction Hn; decompile_compile.
+    - admit.
+      (* TODO
+      set (cx := compile x); assert (compile x = cx) as Hc;
+      [ auto | apply compiles_to_compile in Hc ].
+      inversion Hc; decompile_compile; compiles_to.
+      *)
     - admit.
   Qed.
 
@@ -125,6 +211,8 @@ Section decompile_compile.
         admit.
       + intros.
         admit.
-    - admit.
+    - apply decompiles_to_decompile in IHt; induction IHt;
+      try (simpl; auto; reflexivity);
+      admit.
   Qed.
 End decompile_compile.
